change fin to nat

src/completeness/semantics.lean
@@ -8,25 +8,23 @@ import ..default
 
 open form classical
 
-@[reducible] def wrld (σ : nat) := ctx σ
-
-variable {σ : nat}
+@[reducible] def wrld := set form
 
 /- Kripke models -/
 
 structure model := 
-  (W : set (wrld σ)) 
-  (R : wrld σ → wrld σ → Prop) 
-  (val : fin σ → wrld σ → Prop)
+  (W : set wrld)
+  (R : wrld → wrld → Prop) 
+  (val : ℕ → wrld → Prop)
   (refl : ∀ w ∈ W, R w w)
   (trans : ∀ w ∈ W, ∀ v ∈ W, ∀ u ∈ W, R w v → R v u → R w u)
 
 local attribute [instance] prop_decidable
 
 @[simp]
-def forces_form (M : model) : form σ → wrld σ → Prop
+def forces_form (M : model) : form → wrld → Prop
 |  (#p)   := λ v, M.val p v
-| (bot σ) := λ v, false 
+| (bot) := λ v, false 
 | (p ⊃ q) := λ v, (∀ w ∈ M.W, v ∈ M.W → M.R v w → forces_form p w → forces_form q w)
 | (p & q) := λ v, forces_form p v ∧ forces_form q v
 | (p ∨ q) := λ v, forces_form p v ∨ forces_form q v
@@ -37,18 +35,18 @@ notation w `⊩` `⦃` M `⦄ ` p := forces_form M p w
 
 /- Local logical consequence -/
 
-def forces_ctx (M : model) (Γ : ctx σ) : wrld σ → Prop :=
+def forces_ctx (M : model) (Γ : set form) : wrld → Prop :=
 λ w, ∀ p, p ∈ Γ → forces_form M p w
 
 notation w `⊩` `⦃` M `⦄ ` p := forces_ctx M p w
 
-def sem_csq (Γ : ctx σ) (p : form σ) := 
+def sem_csq (Γ : set form) (p : form) := 
 ∀ (M : model) (w ∈ M.W), (w ⊩⦃M⦄ Γ) → (w ⊩⦃M⦄ p)
 
 notation Γ ` ⊨ᵢ ` p := sem_csq Γ p
 
 /- a helpful lemma -/
 
-lemma ctx_tt_to_subctx_tt {Γ Δ : ctx σ} {M : model} {w : wrld σ} : 
+lemma ctx_tt_to_subctx_tt {Γ Δ : set form} {M : model} {w : wrld} : 
   (w ⊩⦃M⦄ Γ) → Δ ⊆ Γ → (w ⊩⦃M⦄ Δ) :=
 by { intros h s p pmem, apply h, apply s, assumption}
